simulations/simitree/SimModSemFacts0.v
@@ -16,13 +16,14 @@ From ExtLib Require Import
 Require Import Any.
 
 Require Import Mod EventsRed Events.
-Require Import SimGlobal SimGlobalFacts SimInitial SimModSem.
+Require Import SimGlobal SimGlobalFacts SimModSem.
 Require Import Red IRed.
 
 Set Implicit Arguments.
 
 Local Open Scope nat_scope.
 
+(* Adequacy - Part 1. ( Divided to resolve the dependency issue. ) *)
 
 Module TAC.
   Ltac ired_l := try (prw _red_gen 2 0).
@@ -36,6 +37,7 @@ Module TAC.
   Ltac force := ired_both; guclo simg_indC_spec; econs; et.
 End TAC.
 Import TAC.
+
 
 Section SIMMOD.
 
@@ -56,6 +58,56 @@ Section SIMMOD.
   
 End SIMMOD.
 
+Lemma itree_modE_inv R (itr: itree modE R):
+  (exists r, itr = Ret r) \/
+  (exists itr', itr = tau;; itr') \/
+  (exists V (e: coreE V) ktr, itr = v <- trigger e;; ktr v) \/
+  (exists fn args ktr, itr = v <- trigger (Call fn args);; ktr v) \/
+  (exists V run ktr, itr = v <- trigger (@SUpdate V run);; ktr v).
+Proof.
+  ides itr; eauto.
+  right. right. destruct e as [c|[s'|e']].
+  - destruct c. right. left.
+    esplits. rewrite bind_trigger. eauto.
+  - destruct s'. right. right.
+    esplits. rewrite bind_trigger. eauto.
+  - left. esplits. rewrite bind_trigger. eauto.
+Qed.
+
+Section WF.
+  
+  Lemma ModSemR_sim_wf
+    ms_src ms_tgt
+    (SIM : ModSemR.sim ms_src ms_tgt)
+    (WF : ModSem.wf ms_src)
+    :
+    ModSem.wf ms_tgt.
+  Proof.
+    destruct SIM, WF. econs.
+    eapply in_eqlen_nodup_rev; try apply wf_fnsems.
+    { rewrite !map_length. eauto. }
+    i. destruct (alist_find x (ModSem.fnsems ms_src)) eqn: EQS; cycle 1.
+    { apply alist_find_fst_none in EQS. ss. }
+    apply sim_fnsems in EQS. des; subst.
+    apply alist_find_fst_some in EQS. eauto.
+  Qed.
+  
+  Lemma ModR_sim_wf
+    md_src md_tgt
+    (SIM : ModR.sim md_src md_tgt)
+    (WF : Mod.wf md_src)
+    :
+    Mod.wf md_tgt.
+  Proof.
+    destruct WF, SIM, md_src, md_tgt. ss. des. subst.
+    split; eauto.
+    eapply ModSemR_sim_wf; eauto.
+    eapply sim_modsem; eauto using Sk.sort_incl, Sk.sort_wf.
+  Qed.
+
+End WF.
+
+
 
 
 (**** Contextual Refinement on Simulation level ****)
@@ -63,17 +115,12 @@ Section SIMCTX.
 Import ModSem.
 
 Definition wf_lift {world} wf  :=
-  fun (w:world) => 
-  (fun '(src, tgt) => 
-    match (Any.split src), (Any.split tgt) with
-    | Some (l1, r1), Some (l2, r2) => ( wf w (l1, l2) /\ r1 = r2)
-    | _, _ => False
-    end
-  ).
+  fun (w: world) '(src, tgt) => exists st1S st1T st2,
+    src = Any.pair st1S st2 /\ tgt = Any.pair st1T st2 /\
+    wf w (st1S, st1T).
 
 Definition addf f1 f2 : alist gname (Any.t -> itree _ Any.t) :=
     (List.map trans_l f1) ++ (List.map trans_r f2).
-
 
 Lemma sim_ctx_aux {world}
       w wf le
@@ -85,17 +132,14 @@ Lemma sim_ctx_aux {world}
       (TGT: Any.split str = Some (c, a))
 
       (SIM: sim_itree wf le fb fc ol or w (b, itl) (c, itr))
-:
-      @sim_itree world (wf_lift wf) le (addf fb fa) (addf fc fa) ol or w (stl, translate (emb_ run_l) itl) 
-                                              (str, translate (emb_ run_l) itr)
+  :
+  @sim_itree world (wf_lift wf) le (addf fb fa) (addf fc fa) ol or w
+    (stl, translate (emb_ run_l) itl) 
+    (str, translate (emb_ run_l) itr)
 .
 Proof.
-  ginit.
-
-  revert_until wf.
-
+  ginit. revert_until wf.
   gcofix CIH. i.
-
   hexploit SIM. intros SIM'.
 
   remember (b, itl) eqn:PL.
@@ -114,8 +158,9 @@ Proof.
     rewrite translate_emb_ret.
     gstep. apply sim_itree_ret.
     econs; et. esplits; et.
-    unfold wf_lift. rewrite SRC, TGT. split; et.
-
+    eapply Any.split_pair in SRC, TGT. des. subst.
+    r. esplits; eauto.
+    
   - remember (` x : _ <- trigger (Call fn varg);; k_src x). 
     remember (` x : _ <- trigger (Call fn varg);; k_tgt x). 
     remember (b, ` x : _ <- trigger (Call fn varg);; k_src x) eqn:PL.
@@ -135,9 +180,12 @@ Proof.
     try (match goal with
     | |- wf_lift _ _ (_, _) =>  unfold wf_lift; rewrite SRC, TGT; et
     end).
-    all: ii; econs; gfinal; left; ss; des_ifs; try rename WF0 into WF1; inv WF1; eapply CIH; et;
-         specialize (K _ vret _ _ WLE H); pclearbot; apply sim_itree_bot_flag_up; apply K.
-    
+
+    all: eapply Any.split_pair in SRC, TGT; des; subst; rr; esplits; eauto.
+    all: ii; econs; gfinal; left; ss; des; subst; eapply CIH;
+      try rewrite Any.pair_split; eauto;
+      eapply sim_itree_bot_flag_up, K; eauto.
+
   - punfold SIM. inv SIM; (try rewrite ! bind_trigger in H4); (try rewrite ! bind_trigger in H6); clarify.
     + apply inj_pair2 in H0, H1.
       rewrite ! translate_emb_bind, translate_emb_coreE.
@@ -211,7 +259,8 @@ Proof.
       rewrite ! translate_emb_ret.
       gstep. apply sim_itree_ret.
       econs; et. esplits; et.
-      unfold wf_lift. rewrite SRC, TGT. split; et.
+      apply Any.split_pair in SRC, TGT. des; subst.
+      r. esplits; eauto.
     + remember (` x : _ <- trigger (Call fn varg);; k_src x). 
       remember (` x : _ <- trigger (Call fn varg);; k_tgt x). 
       remember (b, ` x : _ <- trigger (Call fn varg);; k_src x) eqn:PL.
@@ -232,8 +281,10 @@ Proof.
           | |- wf_lift _ _ _ => unfold wf_lift; rewrite SRC, TGT; et
           end
       ).
-      all: ii; econs; gfinal; left; ss; des_ifs; try rename WF0 into WF1; inv WF1; eapply CIH; et;
-      specialize (K _ vret _ _ WLE H); pclearbot; apply sim_itree_bot_flag_up; apply K.
+      all: eapply Any.split_pair in SRC, TGT; des; subst; rr; esplits; eauto.
+      all: ii; econs; gfinal; left; ss; des; subst; eapply CIH;
+        try rewrite Any.pair_split; eauto;
+        eapply sim_itree_bot_flag_up, K; eauto.
     + punfold SIM0. inv SIM0; (try rewrite ! bind_trigger in H4); (try rewrite ! bind_trigger in H6); clarify.
       * apply inj_pair2 in H0, H1.
         rewrite ! translate_emb_bind, translate_emb_coreE.
@@ -283,6 +334,43 @@ Proof.
       gfinal. left. eapply CIH; et.
 Qed.
 
+Lemma self_sim_r
+  world le wf fl fr w st1S st1T st2 i
+  (ORD: PreOrder le)
+  (WF: wf w (st1S, st1T): Prop)
+  :
+  sim_itree (@wf_lift world wf) le fl fr false false w
+    (Any.pair st1S st2, translate (emb_ run_r) i)
+    (Any.pair st1T st2, translate (emb_ run_r) i).
+Proof.
+  ginit.
+  assert (exists w1, le w w1 /\ wf w1 (st1S, st1T)).
+  { esplits; eauto. refl. }
+  des. clear WF. revert_until fr.
+  gcofix CIH. i.
+
+  assert (INV := itree_modE_inv i). des; subst.
+  - rewrite translate_emb_ret. gstep. econs.
+    r; esplits; eauto. r; esplits; eauto.
+  - rewrite translate_emb_tau. gstep. do 3 econs.
+    gbase. eauto.
+  - rewrite translate_emb_bind, translate_emb_coreE.
+    destruct e.
+    + gstep. eapply sim_itree_choose_tgt. i. econs. econs. gbase. eauto.
+    + gstep. econs. i. econs. econs. gbase. eauto.
+    + gstep. econs. i. econs. gbase. eauto.
+  - rewrite translate_emb_bind, translate_emb_callE.
+    gstep. econs.
+    { r. esplits; eauto. }
+    i. r in WF. des; subst.
+    econs. gbase. eapply CIH, WF1; eauto.
+    etrans; eauto.
+  - rewrite translate_emb_bind, translate_emb_sE.
+    gstep. econs. econs. econs. gbase.
+    unfold run_r. rewrite !Any.pair_split. grind.
+    eapply CIH, H1; eauto.
+Qed.
+
 Theorem sim_ctx
       ctx ms1 ms2
       (SIM: ModSemR.sim ms1 ms2)
@@ -290,108 +378,58 @@ Theorem sim_ctx
       ModSemR.sim (add ms1 ctx) (add ms2 ctx)
 .
 Proof.
- (* Admitted. *)
+  inv SIM.
+  econs; et.
+  { instantiate (1:= wf_lift wf0).
+    unfold add. s. i. des. subst.
+    edestruct sim_initial; eauto. des.
+    esplits; eauto.
+  }
+  { s. unfold add_fnsems.
+    rewrite !app_length, !map_length, sim_length. eauto.
+  }
+  { s. unfold add_fnsems, trans_l, trans_r. intros fn.
+    rewrite !alist_find_app_o, !alist_find_map. unfold o_map in *.
+    des_ifs. i. eapply sim_miss in Heq1. rewrite Heq1 in Heq2. ss.
+  }
+
+  s. unfold add_fnsems, trans_l, trans_r. i.
+  rewrite !alist_find_app_o in FIND. des_ifs.
+  - rewrite alist_find_map in Heq. unfold o_map in *. des_ifs.
+    exploit sim_fnsems; eauto. i; des.
+    eexists. split.
+    + rewrite alist_find_app_o, alist_find_map, x0. s. eauto.
+    + ii. r in SIMMRS. des; subst.
+      exploit x1; eauto. intro SIM.
+      eapply sim_ctx_aux; try rewrite Any.pair_split; eauto.
+  - rewrite alist_find_map in Heq, FIND. unfold o_map in *. des_ifs.
+    eexists. split.
+    + rewrite alist_find_app_o, alist_find_map.
+      apply sim_miss in Heq1. rewrite Heq1. s.
+      rewrite alist_find_map, Heq0. s. eauto.
+    + ii. r in SIMMRS. des; subst.
+      eapply self_sim_r; eauto.
+Qed.
+
+Lemma sim_ctx_mod
+  ctx md_src md_tgt
+  (SIM: ModR.sim md_src md_tgt)
+  :
+  ModR.sim (Mod.add md_src ctx) (Mod.add md_tgt ctx).
+Proof.
   inv SIM.
   econs; et; cycle 1.
-  { 
-    s. ginit. { eapply cpn7_wcompat. eapply simT_mon. }
-    guclo tbindC_spec. econs.
-    { gfinal. right. eauto. }
-    i. subst.
-    guclo tbindC_spec. econs.
-    { gfinal. right. eapply self_simT; ss. }
-    i. subst.
-    gstep. econs; ss. inv SIM.
-    instantiate (1:= wf_lift wf0). exists x.
-    ss. rewrite! Any.pair_split. eauto.
-  }
-   
-  s. unfold add_fnsems, trans_l, trans_r.
-  apply Forall2_app; eapply Forall2_apply_Forall2; et; cycle 1.
-  - instantiate (1:= eq). induction (fnsems ctx); et.
-  - i. clarify. econs; et. ii; clarify.
-    destruct b. ss.
-    destruct (Any.split mrs_src) eqn: SRC; destruct (Any.split mrs_tgt) eqn:TGT; clarify.
-    2: { destruct p. clarify. }
-    destruct p, p0. des. clarify.
-    assert (exists w1, le w w1 /\ wf0 w1 (t0, t2)).
-    { exists w. splits; et. refl. }
-    clear SIMMRS.
-    des.
-    ginit.
-    revert_until w1.
-    revert w1 w.
-    
-    revert SRC TGT.
-    revert t0 t2 t3.
-    revert mrs_src mrs_tgt.
-    
-    generalize (i y) as it.
-    revert_until wf0.
-    gcofix CIH. i.
-    apply Any.split_pair in SRC. 
-    apply Any.split_pair in TGT.
-    des. clarify.  
-    ides it.
-    + rewrite ! translate_emb_ret.
-      gstep. apply sim_itree_ret.
-      unfold lift_rel. esplits; et.
-      s. rewrite ! Any.pair_split. et.     
-    + rewrite ! translate_emb_tau.
-      gstep. 
-      apply sim_itree_tau_src. apply sim_itree_tau_tgt. 
-      eapply sim_itree_progress; et.
-      gfinal. left. 
-      eapply CIH; et; des; clarify; rewrite ! Any.pair_split; et.
-    + erewrite ! (bisimulation_is_eq _ _ (translate_vis _ _ _ _)).
-      rewrite <- ! bind_trigger.
-      destruct e as [c|[s'|e']].
-      * (* callE *)
-        gstep. destruct c.
-        eapply sim_itree_call; clarify.
-        { s. rewrite ! Any.pair_split. esplits; et. }
-        i. econs. gfinal. left.
-        ss. destruct (Any.split st_src0) eqn: SPL1; destruct (Any.split st_tgt0) eqn: SPL2; clarify.
-        2: { destruct p. clarify. }
-        destruct p, p0, WF.
-        eapply CIH.
-        9: { etrans; et. }
-        all: clarify; et. 
-      * (* sE *)
-         gstep. destruct s'.
-         apply sim_itree_supdate_src. apply sim_itree_supdate_tgt.
-         eapply sim_itree_progress; et.
-         unfold run_r. rewrite ! Any.pair_split.
-         gfinal. left. destruct (run t3). ss. eapply CIH; et; rewrite ! Any.pair_split; et.
-      * (* coreE *)
-        gstep. destruct e'.
-        -- (* Choose *)
-           apply sim_itree_choose_tgt. i. eapply sim_itree_choose_src.
-           eapply sim_itree_progress; et.
-           gfinal. left. eapply CIH; et; rewrite ! Any.pair_split; et.
-        -- (* Take *)
-           apply sim_itree_take_src. i. eapply sim_itree_take_tgt. 
-           eapply sim_itree_progress; et.
-           gfinal. left. eapply CIH; et; rewrite ! Any.pair_split; et.
-        -- (* Syscall *)
-           apply sim_itree_io. i. econs.
-           gfinal. left. eapply CIH; et; rewrite ! Any.pair_split; et.
-  - i. destruct H. r in H. rr in H0. 
-    destruct a, b. econs; et. ss.
-    ii; clarify. ss. 
-    destruct (Any.split mrs_src) eqn: SRC; destruct (Any.split mrs_tgt) eqn:TGT; clarify.
-    2: { destruct p. clarify. }
-    destruct p, p0. des. clarify.
-    specialize H0 with (x:=y) (y:=y) (w:=w) (mrs_src := t0) (mrs_tgt := t2).
-    specialize (H0 eq_refl SIMMRS).
-    eapply sim_ctx_aux; et.
+  { r. ss. unfold Sk.add. ss. rewrite sim_sk. et. }
+  
+  i. ss. hexploit (sim_modsem sk); et.
+  - unfold Sk.incl, Sk.add in *. i. ss.
+    apply SKINCL. rewrite in_app_iff. et.
+  - ii. des. apply sim_ctx; et.
 Qed.
 
 End SIMCTX.
 
-
-(* Adequacy - Part 1. ( Divided to resolve the dependency issue. ) *)
-Section SEMPAIR.
+Section SEMR.
   Variable ms_src: ModSem.t.
   Variable ms_tgt: ModSem.t.
   Definition fl_src := ms_src.(ModSem.fnsems).
@@ -400,15 +438,17 @@ Section SEMPAIR.
   Variable wf: world -> Any.t * Any.t -> Prop.
   Variable le: world -> world -> Prop.
   Hypothesis le_PreOrder: PreOrder le.
-  
-  Hypothesis fnsems_find_iff:
-    forall fn,
-      (<<NONE: alist_find fn ms_src.(ModSem.fnsems) = None>>) \/
-      (exists (f_src f_tgt: _ -> itree _ _),
-          (<<SRC: alist_find fn ms_src.(ModSem.fnsems) = Some f_src>>) /\
-          (<<TGT: alist_find fn ms_tgt.(ModSem.fnsems) = Some f_tgt>>) /\
-          (<<SIM: sim_fsem wf le fl_src fl_tgt f_src f_tgt>>)).
-          
+  Hypothesis sim_initial:
+    forall stS (SAT: ModSem.initial_st ms_src stS),
+    exists w stT, ModSem.initial_st ms_tgt stT /\ wf w (stS, stT).
+  Hypothesis sim_miss : forall fn,
+      alist_find fn (ModSem.fnsems ms_src) = None ->
+      alist_find fn (ModSem.fnsems ms_tgt) = None.
+  Hypothesis sim_fnsems : forall fn fs,
+      alist_find fn (ModSem.fnsems ms_src) = Some fs ->
+      exists ft, alist_find fn (ModSem.fnsems ms_tgt) = Some ft /\
+      sim_fsem wf le (ModSem.fnsems ms_src) (ModSem.fnsems ms_tgt) fs ft.
+    
   Variant g_lift_rel
           (w0: world) st_src st_tgt: Prop :=
   | g_lift_rel_intro
@@ -417,27 +457,18 @@ Section SEMPAIR.
       (MN: wf w1 (st_src, st_tgt))
   .
 
-  Variant my_r0:
-    forall R0 R1 (RR: R0 -> R1 -> Prop), bool -> bool -> (itree coreE R0) -> (itree coreE R1) -> Prop :=
-  | my_r0_intro
-      w0
-      (itr_src itr_tgt: itree modE Any.t)
-      st_src st_tgt o_src o_tgt
-      (SIM: sim_itree wf le fl_src fl_tgt o_src o_tgt w0 (st_src, itr_src) (st_tgt, itr_tgt))
-      (* (STATE: forall mn' (MN: mn <> mn'), Any.t mn' = Any.t mn') *)
+  Lemma sim_itree_simg
+    w0 itr_src itr_tgt st_src st_tgt o_src o_tgt
+    (SIM: sim_itree wf le fl_src fl_tgt o_src o_tgt w0 (st_src, itr_src) (st_tgt, itr_tgt))
     :
-      my_r0 (fun '(st_src, ret_src) '(st_tgt, ret_tgt) =>
+    simg (fun '(st_src, ret_src) '(st_tgt, ret_tgt) =>
                 g_lift_rel w0 st_src st_tgt /\ ret_src = ret_tgt)
-            o_src o_tgt
-            (interp_modE (ModSem.prog ms_src) (itr_src) st_src)
-            (interp_modE (ModSem.prog ms_tgt) (itr_tgt) st_tgt)
-  .
-
-  Let sim_lift: my_r0 <7= simg.
+    o_src o_tgt
+    (interp_modE (ModSem.prog ms_src) itr_src st_src)
+    (interp_modE (ModSem.prog ms_tgt) itr_tgt st_tgt).
   Proof.
-    ginit.
-    { i. eapply cpn7_wcompat; eauto with paco. }
-    gcofix CIH. i. destruct PR.
+    ginit. revert_until sim_initial.
+    gcofix CIH. i.
     unfold sim_itree in SIM.
     remember (st_src, itr_src).
     remember (st_tgt, itr_tgt).
@@ -451,23 +482,22 @@ Section SEMPAIR.
     revert o_src o_tgt w p p0 SIM.
     eapply (@sim_itree_ind world wf le fl_src fl_tgt Any.t Any.t (lift_rel wf le w0 (@eq Any.t)) P); subst P; ss; i; clarify.
     - rr in RET. des. step. splits; auto. econs; et.
-    - hexploit (fnsems_find_iff fn). i. des.
-      { steps. rewrite NONE. unfold unwrapU, triggerUB. grind. step. ss. }
-
-      { hexploit (SIM (varg) (varg)); et. i. des. ired_both. 
-        steps. grind. rewrite SRC. rewrite TGT. unfold unwrapU. ired_both.
-        apply simg_progress_flag.
-        guclo bindC_spec. econs.
-        { gbase. eapply CIH. econs; ss. grind. et. }
-        { i. ss. destruct vret_src, vret_tgt. des; clarify. inv SIM0.
-          hexploit K; et. i. des. pclearbot. ired_both.
-          steps. gbase. eapply CIH. econs; et.
-          eapply sim_itree_bot_flag_up. et.           
-        }
-      }
+    - destruct (alist_find fn fl_src) eqn: EQ; cycle 1.
+      { steps. fold fl_src fl_tgt.
+        rewrite EQ. unfold unwrapU, triggerUB. grind. step. ss. }
+      hexploit sim_fnsems; eauto. i; des.
+      hexploit (H0 (varg) (varg)); et. i.
+      steps. fold fl_src fl_tgt in *. rewrite EQ, H. unfold unwrapU. steps.
+      apply simg_progress_flag.
+      guclo bindC_spec. econs.
+      { gbase. eapply CIH; et. }
+      i. ss. destruct vret_src, vret_tgt. des; clarify. inv SIM.
+      hexploit K; et. i. steps.
+      gbase. eapply CIH; et. 
+      eapply sim_itree_bot_flag_up. et.           
     - step. i. subst. apply simg_progress_flag.
       hexploit (K x_tgt). i. des. pclearbot.
-      steps. gbase. eapply CIH. econs; et.
+      steps. gbase. eapply CIH; et.
     - steps. unfold fl_src in FUN. rewrite FUN. grind.
       rewrite <- interp_modE_bind.
       eapply IH; et.
@@ -482,50 +512,75 @@ Section SEMPAIR.
     - des. force. exists x. steps. eapply IH; eauto.
     - steps. destruct run. steps. eapply IH; eauto.
     - steps. destruct run. steps. eapply IH; eauto.
-    - eapply simg_progress_flag. gbase. eapply CIH. econs; eauto.
+    - eapply simg_progress_flag. gbase. eapply CIH; eauto.
   Qed.
-
-  Hypothesis INIT:
-    simT (fun x y => exists w, wf w (x, y)) false false ms_src.(ModSem.initial_st) ms_tgt.(ModSem.initial_st).
 
   Lemma adequacy_local_aux (P Q: Prop)
-        (* (wf: world -> W -> Prop)  *)
-        (WF: Q -> P)
+    (LE: Q -> P)
     :
-      (Beh.of_program (ModSem.compile ms_tgt (Some P)))
-      <1=
-      (Beh.of_program (ModSem.compile ms_src (Some Q))).
+    (Beh.of_program (ModSem.compile ms_tgt P))
+    <1=
+    (Beh.of_program (ModSem.compile ms_src Q)).
   Proof. 
     eapply adequacy_global_itree; ss.
-    (* inv INIT.  *)
-    des. ginit.
-    { eapply cpn7_wcompat; eauto with paco. }
+    ginit.
     unfold ModSem.initial_itr, assume. generalize "CCR_init" as fn. i.
-    hexploit (fnsems_find_iff fn). i. des.
-    { 
-      esplits. guclo bindC_spec. econs.
-      { steps. force. exists (WF x). steps. ss. }
-      i. grind. 
-      unfold ITree.map, unwrapU, triggerUB.
-      steps. guclo bindC_spec. econs.
-      { gfinal. right. eapply adequacy_initial. eapply INIT. }
-      i. rewrite NONE. steps. ss.
-    }
-    {
-      esplits. guclo bindC_spec. econs.
-      { steps. force. exists (WF x). steps. ss. }
-      i. grind.
-      unfold ITree.map. steps. guclo bindC_spec. econs.
-      { gfinal. right. eapply adequacy_initial. eapply INIT. }
-      i. unfold unwrapU. rewrite SRC, TGT. grind.
-      inv SIM0.
-      guclo bindC_spec. econs.
-      {
-        hexploit (SIM ()↑ ()↑); et; cycle 1. i.
-        gfinal. right. eapply sim_lift. econs; eauto.
-      }  
-      { i. destruct vret_src0, vret_tgt1. des; clarify. steps. }
-    }
+
+    guclo bindC_spec. econs.
+    { step. force. eexists; eauto. step. ss. }
+    i. subst. ss. unfold ITree.map. grind.
+
+    steps. hexploit sim_initial; eauto. i; des.
+    force. eexists. force. eexists; eauto. steps.
+
+    fold fl_src fl_tgt.
+    destruct (alist_find fn fl_src) eqn: EQ; cycle 1.
+    { grind. unfold triggerUB. grind. steps. ss. }
+
+    hexploit sim_fnsems; eauto. i; des.
+    fold fl_src fl_tgt in *.
+    rewrite H1. grind.
+    guclo bindC_spec. econs.
+    { gstep. econs; eauto. gfinal. right.
+      eapply sim_itree_simg. eapply H2; eauto. }
+    i. steps.
+    destruct vret_src, vret_tgt0. des; subst; eauto.
   Qed.
 
-End SEMPAIR.
+End SEMR.
+
+Section ADEQUACY.
+
+  Lemma adequacy_modsem
+    ms_src ms_tgt (Q P: Prop)
+    (SIM: ModSemR.sim ms_src ms_tgt)
+    (WF : ModSem.wf ms_src)
+    (LE: Q -> P)
+    :
+    <<REF: Beh.of_program (ModSem.compile ms_tgt P) <1= Beh.of_program (ModSem.compile ms_src Q) >>.
+  Proof.
+    ii. destruct SIM. eapply adequacy_local_aux; eauto.
+  Qed.
+  
+  Lemma adequacy_mod
+    md_src md_tgt
+    (SIM: ModR.sim md_src md_tgt)
+    :
+    <<REF: Beh.of_program (Mod.compile md_tgt) <1= Beh.of_program (Mod.compile md_src) >>
+    .
+  Proof.
+    destruct (classic (Mod.wf md_src)) as [WF|]; cycle 1.
+    { intros x.
+      eapply adequacy_global_itree.
+      unfold ModSem.initial_itr, assume.
+      ginit. grind. gstep. econs; eauto. i. ss.
+    }
+
+    assert (SIM0 := SIM).
+    destruct WF, SIM0, md_src, md_tgt. ss. des. subst.
+    apply Sk.sort_wf in H0.
+    hexploit sim_modsem; eauto using Sk.sort_incl; try reflexivity.
+    ii. eapply adequacy_modsem, PR; eauto using ModR_sim_wf.
+  Qed.
+
+End ADEQUACY.
