simulations/ctxrefine/ModFacts.v
@@ -1,0 +1,776 @@
+Require Import Coqlib.
+Require Export sflib.
+Require Export ITreelib.
+Require Import STS Behavior.
+Require Import Mod EventsRed Events.
+Require Import SimGlobal SimGlobalFacts.
+Require Import Skeleton.
+Require Import STS Behavior.
+Require Import Any.
+Require Import Red IRed.
+Require Import SimModSem SimModSemFacts0.
+
+Require Import Behavior.
+Require Import Relation_Definitions.
+
+(*** TODO: export these in Coqlib or Universe ***)
+Require Import Relation_Operators.
+Require Import RelationPairs.
+From ITree Require Import
+     Events.MapDefault
+     TranslateFacts.
+From ExtLib Require Import
+     Core.RelDec
+     Structures.Maps
+     Data.Map.FMapAList.
+Require Import Any.
+
+
+Set Implicit Arguments.
+
+Import TAC.
+
+Module ModSemFacts.
+Import ModSem.
+
+Section EMPTY.
+
+  Inductive empty_emb : IFun modE modE -> Prop := 
+    | empty_emb_intro : empty_emb emb_l
+  .
+
+  Inductive empty_ems : itree modE Any.t -> itree modE Any.t -> Prop := 
+    | empty_ems_intro emb_l it (EMB: empty_emb emb_l) :
+        empty_ems it (translate emb_l it).    
+
+  Definition empty_st (stp: Any.t * Any.t) : Prop :=
+    exists a, fst stp = a /\ snd stp = Any.pair a tt↑.
+
+  Definition empty_rev_st (stp: Any.t * Any.t) : Prop :=
+    exists a, fst stp = Any.pair a tt↑ /\ snd stp = a.
+                              
+  Lemma add_empty_aux
+          fl fr itl itr stl str (w: unit)
+          (EMPTY: empty_ems itl itr)
+          (STATE: empty_st (stl, str))
+
+    :
+        sim_itree (fun _ => empty_st) top2 fl fr false false w (stl, itl) (str, itr)
+  .
+  Proof.
+    destruct EMPTY, STATE. des. ss.
+    unfold empty_st.
+    ginit. 
+    generalize it as itr. 
+    clarify.
+    generalize x as a.
+    gcofix CIH. i.
+    rewrite (itree_eta_ itr).
+    destruct (observe itr).
+    - (* Ret *)
+      erewrite ! (bisimulation_is_eq _ _ (translate_ret _ _)).
+      gstep. apply sim_itree_ret.
+      unfold lift_rel. 
+      exists tt. splits; et.
+    - (* Tau *)
+      erewrite ! (bisimulation_is_eq _ _ (translate_tau _ _)).
+      gstep. 
+      apply sim_itree_tau_src. apply sim_itree_tau_tgt. 
+      eapply sim_itree_progress; et.
+      gfinal. left. eapply CIH; et.
+    - (* Vis *)
+      erewrite ! (bisimulation_is_eq _ _ (translate_vis _ _ _ _)).
+      rewrite <- ! bind_trigger.
+      destruct e as [c|[s|e]].
+      + (* callE *)
+        gstep. destruct c, EMB. 
+        apply sim_itree_call; clarify.
+        -- exists a; et.
+        -- i. destruct WF, H. ss. clarify.
+           econs. gfinal. left. eapply CIH.
+      + (* sE *)
+        gstep. destruct s, EMB.
+        apply sim_itree_supdate_src. apply sim_itree_supdate_tgt.
+        eapply sim_itree_progress; et.
+        unfold run_l, run_r. rewrite ! Any.pair_split.
+        gfinal. left. destruct (run a). eapply CIH.
+      + (* eventE *)
+        gstep. destruct e, EMB.
+        * (* Choose *)
+          apply sim_itree_choose_tgt. i. eapply sim_itree_choose_src. 
+          eapply sim_itree_progress; et.
+          gfinal. left. eapply CIH.
+        * (* Take *)
+          apply sim_itree_take_src. i. eapply sim_itree_take_tgt.
+          eapply sim_itree_progress; et.
+          gfinal. left. eapply CIH. 
+        * (* Syscall *)
+          apply sim_itree_io. i.
+          econs. gfinal. left. eapply CIH. 
+  Qed.
+
+  Lemma add_empty_rev_aux
+          fl fr itl itr stl str (w: unit)
+          (EMPTY: empty_ems itr itl)
+          (STATE: empty_rev_st (stl, str))
+    :
+        sim_itree (fun _ => empty_rev_st) top2 fl fr false false w (stl, itl) (str, itr)
+  .
+  Proof.
+    destruct EMPTY, STATE. des. ss.
+    unfold empty_rev_st.
+    ginit.
+    generalize it as itr.
+    clarify.
+    generalize x as a.
+    gcofix CIH. i.
+    ides itr.
+    - (* Ret *)
+      erewrite ! (bisimulation_is_eq _ _ (translate_ret _ _)).
+      gstep. apply sim_itree_ret.
+      unfold lift_rel.
+      exists tt. splits; et.
+    - (* Tau *)
+      erewrite ! (bisimulation_is_eq _ _ (translate_tau _ _)).
+      gstep.
+      apply sim_itree_tau_src. apply sim_itree_tau_tgt.
+      eapply sim_itree_progress; et.
+      gfinal. left. eapply CIH; et.
+    - (* Vis *)
+      erewrite ! (bisimulation_is_eq _ _ (translate_vis _ _ _ _)).
+      rewrite <- ! bind_trigger.
+      destruct e as [c|[s|e]].
+      + (* callE *)
+        gstep. destruct c, EMB.
+        apply sim_itree_call; clarify.
+        -- exists a; et.
+        -- i. destruct WF, H. ss. clarify.
+           econs. gfinal. left. eapply CIH.
+      + (* sE *)
+        gstep. destruct s, EMB.
+        apply sim_itree_supdate_src. apply sim_itree_supdate_tgt.
+        eapply sim_itree_progress; et.
+        unfold run_l, run_r. rewrite ! Any.pair_split.
+        gfinal. left. destruct (run a). eapply CIH.
+      + (* eventE *)
+        gstep. destruct e, EMB.
+        * (* Choose *)
+          apply sim_itree_choose_tgt. i. eapply sim_itree_choose_src.
+          eapply sim_itree_progress; et.
+          gfinal. left. eapply CIH.
+        * (* Take *)
+          apply sim_itree_take_src. i. eapply sim_itree_take_tgt.
+          eapply sim_itree_progress; et.
+          gfinal. left. eapply CIH.
+        * (* Syscall *)
+          apply sim_itree_io. i.
+          econs. gfinal. left. eapply CIH.
+  Qed.        
+    
+  Theorem add_empty
+        ms
+        (P0 P1: Prop) (IMPL: P1 -> P0)
+        (WF: wf ms)
+    :
+    ModSemR.sim ms (add ms empty)
+  .
+  Proof.
+    econs.
+    { instantiate (1:= fun (_:()) _ => True). econs; ii; subst; eauto. }
+    { instantiate (1:= fun _ => empty_st).
+      i. esplits; rr; esplits; rr; eauto. exact tt.
+    }
+    { s. unfold add_fnsems. rewrite !app_length, !map_length. s. nia. }
+    { i. apply alist_find_fst_none in MISS. apply alist_find_fst_notin.
+      ss. unfold add_fnsems in *. ii. apply MISS. clear MISS.
+      ss. rewrite app_nil_r, List.map_map, fun_fst_trans_l in *. eauto.
+    }
+
+    s. unfold add_fnsems. ss. i. rewrite app_nil_r.
+    unfold trans_l at 1. rewrite !alist_find_map, FIND. s.
+    esplits; eauto.
+    ii. subst. rr in SIMMRS. des; ss; subst.
+    eapply add_empty_aux; eauto.
+    - econs. econs.
+    - econs. s; esplits; eauto.
+  Qed.
+
+  Theorem add_empty_rev
+        ms
+        (P0 P1: Prop) (IMPL: P1 -> P0)
+        (WF: wf ms)
+    :
+    ModSemR.sim (add ms empty) ms
+  .
+  Proof.
+    econs.
+    { instantiate (1:= fun (_:()) _ => True). econs; ii; subst; eauto. }
+    { instantiate (1:= fun _ => empty_rev_st).
+      i. rr in SAT. des; subst. rr in SAT1; subst.
+      esplits; rr; esplits; rr; eauto. exact tt.
+    }
+    { s. unfold add_fnsems. rewrite !app_length, !map_length. s. nia. }
+    { i. apply alist_find_fst_none in MISS. apply alist_find_fst_notin.
+      ss. unfold add_fnsems in *. ii. apply MISS. clear MISS.
+      ss. rewrite app_nil_r, List.map_map, fun_fst_trans_l in *. eauto.
+    }
+
+    s. unfold add_fnsems. ss. i. rewrite app_nil_r in *.
+    unfold trans_l in FIND. rewrite !alist_find_map in FIND.
+    unfold o_map in *. des_ifs. esplits; eauto.
+    ii. subst. rr in SIMMRS. des; ss; subst.
+    eapply add_empty_rev_aux; eauto.
+    - econs. econs.
+    - econs. s; esplits; eauto.
+  Qed.
+  
+End EMPTY.
+
+
+Section COMM.
+
+  Inductive comm_emb : IFun modE modE -> IFun modE modE -> Prop := 
+    |comm_emb_1 : comm_emb emb_l emb_r
+    |comm_emb_2 : comm_emb emb_r emb_l
+  .
+
+  Inductive comm_ems : itree modE Any.t -> itree modE Any.t -> Prop := 
+    | comm_ems_intro emb_l emb_r it (EMB: comm_emb emb_l emb_r) :
+        comm_ems (translate emb_l it) (translate emb_r it).    
+
+  Definition comm_st (stp: Any.t * Any.t) : Prop :=
+    exists a b, fst stp = Any.pair a b /\ 
+    snd stp = Any.pair b a.
+
+  Lemma add_comm_aux
+        fl fr itl itr stl str (w: unit)
+        (COMM: comm_ems itl itr)
+        (STATE: comm_st (stl, str))
+  :
+      sim_itree (fun _ => comm_st) top2 fl fr false false w (stl, itl) (str, itr).
+  Proof.   
+    destruct COMM, STATE. des. ss.
+    ginit. 
+    generalize it as itr. 
+    clarify.
+    generalize x as a0.
+    generalize b as b0.
+    gcofix CIH. i.
+    rewrite (itree_eta_ itr).
+    destruct (observe itr).
+    - erewrite ! (bisimulation_is_eq _ _ (translate_ret _ _)).
+      gstep. apply sim_itree_ret.
+      unfold lift_rel. 
+      eexists; et. splits; et.
+      unfold comm_st. exists a0, b0; et.
+    - erewrite ! (bisimulation_is_eq _ _ (translate_tau _ _)).
+      gstep. 
+      apply sim_itree_tau_src. apply sim_itree_tau_tgt. 
+      eapply sim_itree_progress; et.
+      gfinal. left. eapply CIH; et.
+    - erewrite ! (bisimulation_is_eq _ _ (translate_vis _ _ _ _)).
+      rewrite <- ! bind_trigger.
+      destruct e as [c|[s|e]].
+      + (* callE *)
+        gstep. destruct c, EMB. 
+        (* SIMPLIFY BELOW *)
+        * apply sim_itree_call; clarify.
+          -- exists a0, b0; et.
+          -- i. unfold comm_st in WF. des. ss. clarify.
+             econs. gfinal. left. eapply CIH.
+        * apply sim_itree_call; clarify.
+          -- eexists a0, b0; et.
+          -- i. unfold comm_st in WF. des. ss. clarify.
+             econs. gfinal. left. eapply CIH.
+      + (* sE *)
+        gstep. destruct s, EMB.
+        * apply sim_itree_supdate_src. apply sim_itree_supdate_tgt.
+          eapply sim_itree_progress; et.
+          unfold run_l, run_r. rewrite ! Any.pair_split.
+          gfinal. left. destruct (run a0). eapply CIH.
+        * apply sim_itree_supdate_src. apply sim_itree_supdate_tgt.
+          eapply sim_itree_progress; et.
+          unfold run_l, run_r. rewrite ! Any.pair_split.
+          gfinal. left. destruct (run b0). eapply CIH.  
+      + (* eventE *)
+        gstep. destruct e, EMB.
+        (* Choose *)
+        * apply sim_itree_choose_tgt. i. eapply sim_itree_choose_src.
+          eapply sim_itree_progress; et.
+          gfinal. left. eapply CIH.
+        * apply sim_itree_choose_tgt. i. eapply sim_itree_choose_src.
+          eapply sim_itree_progress; et.
+          gfinal. left. eapply CIH.
+        (* Take *)
+        * apply sim_itree_take_src. i. eapply sim_itree_take_tgt.
+          eapply sim_itree_progress; et.
+          gfinal. left. eapply CIH. 
+        * apply sim_itree_take_src. i. eapply sim_itree_take_tgt.
+          eapply sim_itree_progress; et.
+          gfinal. left. eapply CIH. 
+        (* Syscall *)
+        * apply sim_itree_io. i.
+          econs. gfinal. left. eapply CIH. 
+        * apply sim_itree_io. i.
+          econs. gfinal. left. eapply CIH.
+  Qed. 
+
+  Theorem add_comm
+    ms0 ms1
+    (P0 P1: Prop) (IMPL: P1 -> P0)
+    (WF: wf (add ms1 ms0))
+    :
+    ModSemR.sim (add ms1 ms0) (add ms0 ms1).
+  Proof.
+    econs.
+    { instantiate (1:= fun (_:()) _ => True). econs; ii; subst; eauto. }
+    { instantiate (1:= fun _ => comm_st).
+      i. rr in SAT. des. subst.
+      esplits; rr; esplits; eauto. exact tt.
+    }
+    { s. unfold add_fnsems. rewrite !app_length, !map_length. nia. }
+    { i. apply alist_find_fst_none in MISS. apply alist_find_fst_notin.
+      ss. unfold add_fnsems in *. ii. apply MISS. clear MISS.
+      rewrite !map_app, !List.map_map, fun_fst_trans_l, fun_fst_trans_r in *.
+      apply in_or_app. apply in_app_or in H. des; eauto.
+    }
+
+    s. unfold add_fnsems, trans_l, trans_r. intros fn.
+    rewrite ! alist_find_app_o, ! alist_find_map.
+    destruct (alist_find fn (fnsems ms0)) eqn:MS0;
+      destruct (alist_find fn (fnsems ms1)) eqn: MS1; s; i; ss.
+    + inv FIND. exfalso.
+      apply alist_find_fst_some in MS0, MS1.
+      eapply NoDup_app_disjoint; [|apply MS1|apply MS0].
+      destruct WF. ss. unfold add_fnsems in *.
+      rewrite !map_app, !List.map_map, fun_fst_trans_l, fun_fst_trans_r in *; ss.
+    + inv FIND. esplits; eauto.
+      ii. subst. hexploit add_comm_aux; eauto. econs. econs.
+    + inv FIND. esplits; eauto.
+      ii. subst. hexploit add_comm_aux; eauto. econs. econs.
+  Qed.
+
+End COMM.
+
+Section ASSOC.
+
+  Inductive assoc_emb : IFun modE modE -> IFun modE modE -> Prop := 
+    |assoc_emb_1 : assoc_emb emb_l (emb_l >>> emb_l)
+    |assoc_emb_2 : assoc_emb (emb_l >>> emb_r ) (emb_r >>> emb_l)
+    |assoc_emb_3 : assoc_emb (emb_r >>> emb_r) emb_r
+  .
+
+  Inductive assoc_ems : itree modE Any.t -> itree modE Any.t -> Prop := 
+    | assoc_ems_intro emb_l emb_r it (EMB: assoc_emb emb_l emb_r) :
+        assoc_ems (translate emb_l it) (translate emb_r it).
+     
+  Definition assoc_st (stp: Any.t * Any.t) : Prop :=
+    exists a b c, fst stp = Any.pair a (Any.pair b c) /\ 
+    snd stp = Any.pair (Any.pair a b) c
+  .
+
+  Lemma add_assoc_aux
+        fl fr itl itr stl str (w: unit)
+        (ASSOC: assoc_ems itl itr)
+        (STATE: assoc_st (stl, str))
+    :
+      sim_itree (fun _ => assoc_st) top2 fl fr false false w (stl, itl) (str, itr).
+  Proof.
+    destruct ASSOC, STATE. des. ss.
+    (* unfold assoc_st. *)
+    ginit. 
+    generalize it as itr. 
+    clarify.
+    generalize x as a0.
+    generalize b as b0.
+    generalize c as c0.
+    gcofix CIH. i.
+    rewrite (itree_eta_ itr).
+    destruct (observe itr).
+    - erewrite ! (bisimulation_is_eq _ _ (translate_ret _ _)).
+      gstep. apply sim_itree_ret.
+      unfold lift_rel. 
+      exists tt. splits; et.
+      unfold assoc_st. exists a0, b0, c0; et.
+    - erewrite ! (bisimulation_is_eq _ _ (translate_tau _ _)).
+      gstep. 
+      apply sim_itree_tau_src. apply sim_itree_tau_tgt. 
+      eapply sim_itree_progress; et.
+      gfinal. left. eapply CIH; et.
+    - erewrite ! (bisimulation_is_eq _ _ (translate_vis _ _ _ _)).
+      rewrite <- ! bind_trigger.
+      destruct e as [c'|[s|e]].
+      + (* callE *)
+        gstep. destruct c', EMB. 
+        (* SIMPLIFY BELOW *)
+        * apply sim_itree_call; clarify.
+          -- exists a0, b0, c0; et.
+          -- i. destruct WF, H, H, H. ss. clarify.
+          econs. gfinal. left. eapply CIH.
+        * apply sim_itree_call; clarify.
+          -- eexists a0, b0, c0; et.
+          -- i. unfold assoc_st in WF. des. ss. clarify.
+            econs. gfinal. left. eapply CIH.
+        * apply sim_itree_call; clarify.
+          -- eexists a0, b0, c0; et.
+          -- i. unfold assoc_st in WF. des. ss. clarify.
+            econs. gfinal. left. eapply CIH. 
+      + (* sE *)
+        gstep. destruct s, EMB.
+        * apply sim_itree_supdate_src. apply sim_itree_supdate_tgt.
+          eapply sim_itree_progress; et.
+          unfold run_l, run_r. rewrite ! Any.pair_split.
+          gfinal. left. destruct (run a0). eapply CIH.
+        * apply sim_itree_supdate_src. apply sim_itree_supdate_tgt.
+          eapply sim_itree_progress; et.
+          unfold run_l, run_r. rewrite ! Any.pair_split.
+          gfinal. left. destruct (run b0). eapply CIH.
+        * apply sim_itree_supdate_src. apply sim_itree_supdate_tgt.
+          eapply sim_itree_progress; et.
+          unfold run_l, run_r. rewrite ! Any.pair_split.
+          gfinal. left. destruct (run c0). eapply CIH.        
+      + (* eventE *)
+        gstep. destruct e, EMB.
+        (* Choose *)
+        * apply sim_itree_choose_tgt. i. eapply sim_itree_choose_src.
+          eapply sim_itree_progress; et.
+          gfinal. left. eapply CIH.
+        * apply sim_itree_choose_tgt. i. eapply sim_itree_choose_src.
+          eapply sim_itree_progress; et.
+          gfinal. left. eapply CIH.
+        * apply sim_itree_choose_tgt. i. eapply sim_itree_choose_src.
+          eapply sim_itree_progress; et.
+          gfinal. left. eapply CIH.
+        (* Take *)
+        * apply sim_itree_take_src. i. eapply sim_itree_take_tgt.
+          eapply sim_itree_progress; et.
+          gfinal. left. eapply CIH. 
+        * apply sim_itree_take_src. i. eapply sim_itree_take_tgt.
+          eapply sim_itree_progress; et.
+          gfinal. left. eapply CIH. 
+        * apply sim_itree_take_src. i. eapply sim_itree_take_tgt.
+          eapply sim_itree_progress; et.
+          gfinal. left. eapply CIH.
+        (* Syscall *)
+        * apply sim_itree_io. i.
+          econs. gfinal. left. eapply CIH. 
+        * apply sim_itree_io. i.
+          econs. gfinal. left. eapply CIH.
+        * apply sim_itree_io. i.
+          econs. gfinal. left. eapply CIH.
+  Qed.
+
+  Theorem add_assoc
+          ms0 ms1 ms2
+          (P0 P1: Prop) (IMPL: P1 -> P0)
+          (WF: wf (add ms0 (add ms1 ms2)))
+    :
+    ModSemR.sim (add ms0 (add ms1 ms2)) (add (add ms0 ms1) ms2).
+  Proof. 
+    econs.
+    { instantiate (1:= fun (_:()) _ => True). econs; ii; subst; eauto. }
+    { instantiate (1:= fun _ => assoc_st).
+      i. rr in SAT. des. subst. rr in SAT1. des; subst.
+      esplits; eauto.
+      - exact tt.
+      - rr. esplits; eauto. rr. esplits; eauto.
+      - rr. esplits; eauto.
+    }
+    { s. unfold add_fnsems. rewrite !app_length, !map_length.
+      s. unfold add_fnsems. rewrite !app_length, !map_length. nia.
+    }
+    { i. apply alist_find_fst_none in MISS. apply alist_find_fst_notin.
+      ss. unfold add_fnsems in *. ss. unfold add_fnsems in *. 
+      ii. apply MISS. clear MISS.
+      rewrite !map_app, !List.map_map in *.
+      apply in_app_or in H. des.
+      - apply in_app_or in H. des.
+        + apply in_or_app. left.
+          rewrite fun_fst_trans_l, fun_fst_trans_l_l in *. eauto.
+        + apply in_or_app. right. apply in_or_app. left.
+          rewrite !fun_fst_trans_l_r, !fun_fst_trans_r_l in *. eauto.
+      - apply in_or_app. right. apply in_or_app. right.
+        rewrite !fun_fst_trans_r, !fun_fst_trans_r_r in *. eauto.
+    }
+
+    s. unfold add_fnsems, trans_l, trans_r. intros fn.
+    rewrite ! alist_find_app_o, ! alist_find_map.
+    destruct (alist_find fn (fnsems ms0)) eqn:MS0;
+      destruct (alist_find fn (fnsems ms1)) eqn: MS1; s; i; ss.
+    + inv FIND. exfalso.
+      apply alist_find_fst_some in MS0, MS1.
+      eapply NoDup_app_disjoint; [|apply MS0|apply MS1].
+      destruct WF. do 2 (ss; unfold add_fnsems in *).
+      rewrite !map_app, !List.map_map in *.
+      rewrite app_assoc in wf_fnsems0. apply nodup_app_l in wf_fnsems0.
+      rewrite fun_fst_trans_l, fun_fst_trans_r_l in *. eauto.
+    + inv FIND. unfold add_fnsems, trans_l.
+      rewrite alist_find_app_o, alist_find_map, MS0. s.
+      esplits; eauto.
+      ii. subst. hexploit add_assoc_aux; eauto.
+      erewrite <- !(@bisimulation_is_eq _ _ _ _ (@translate_cmpE _ _ _ _ _ _ _)).
+      econs. econs.
+    + unfold add_fnsems, trans_l, trans_r in *.
+      rewrite !alist_find_app_o, !alist_find_map, !MS0, !MS1 in *. ss.
+      inv FIND. esplits; eauto.
+      ii. subst. hexploit add_assoc_aux; eauto.
+      erewrite <- !(@bisimulation_is_eq _ _ _ _ (@translate_cmpE _ _ _ _ _ _ _)).
+      econs. econs.
+    + unfold add_fnsems, trans_l, trans_r in *.
+      rewrite !alist_find_app_o, !alist_find_map, !MS0, !MS1 in *. ss.
+      destruct (alist_find fn (fnsems ms2)) eqn: MS2; ss.
+      inv FIND. esplits; eauto.
+      ii. subst. hexploit add_assoc_aux; eauto.
+      erewrite <- !(@bisimulation_is_eq _ _ _ _ (@translate_cmpE _ _ _ _ _ _ _)).
+      econs. econs.
+  Qed.
+
+End ASSOC.
+
+End ModSemFacts.
+
+Module ModFacts.
+Import Mod.
+Section BEH.
+
+Context `{Sk.ld}.
+
+Theorem add_comm
+        md0 md1
+  :
+    <<COMM: Beh.of_program (compile (add md0 md1)) <1= Beh.of_program (compile (add md1 md0))>>
+.
+
+Proof.
+  ii. unfold compile in *.
+  destruct (classic (ModSem.wf (enclose (add md1 md0)) /\ Sk.wf (sk (add md1 md0)))).
+  2: { eapply ModSem.initial_itr_not_wf. ss. }
+  ss. des. assert (SK: Sk.wf (Sk.add (sk md0) (sk md1))).
+  { apply Sk.wf_comm. auto. }
+  rewrite Sk.add_comm; et.
+  eapply ModSemFacts.add_comm; [| |et].
+  { i. split; auto. unfold enclose. ss. rewrite Sk.add_comm; et.
+    inv H2. inv H3. econs; ss.
+    unfold ModSem.add_fnsems in *.
+    rewrite ! List.map_app in *.
+    rewrite ! List.map_map in *.
+    rewrite fun_fst_trans_l in *.
+    rewrite fun_fst_trans_r in *.
+    eapply nodup_comm. et.
+  }
+  { rewrite Sk.add_comm; et. }
+Qed.
+
+Theorem add_assoc
+        md0 md1 md2
+  :
+    <<ASSOC: Beh.of_program (compile (add (add md0 md1) md2)) <1=
+            Beh.of_program (compile (add md0 (add md1 md2)))>>
+.
+Proof. 
+  ii. unfold compile in *.
+  destruct (classic (ModSem.wf (enclose (add md0 (add md1 md2))) /\ Sk.wf (sk (add md0 (add md1 md2))))).
+  2: { eapply ModSem.initial_itr_not_wf. ss. }
+  ss. des. assert (SK: Sk.wf (Sk.add (Sk.add (sk md0) (sk md1)) (sk md2))).
+  { rewrite <- Sk.add_assoc. apply H1. }
+  eapply ModSemFacts.add_assoc; [ |et|rewrite Sk.add_assoc;et].
+  i. split; et. unfold enclose. ss.
+  rewrite <- Sk.add_assoc.
+  inv H2. inv H3. econs.
+  repeat (ss; unfold ModSem.add_fnsems in *; rewrite ! List.map_app in *; rewrite ! List.map_map in *).
+  rewrite fun_fst_trans_l in *.
+  rewrite fun_fst_trans_r in *.
+  rewrite fun_fst_trans_l_l in *.
+  rewrite fun_fst_trans_l_r in *.
+  rewrite fun_fst_trans_r_l in *.
+  rewrite fun_fst_trans_r_r in *.
+  rewrite <- app_assoc. apply wf_fnsems.
+Qed.
+
+Theorem add_assoc_rev
+        md0 md1 md2
+  :
+    <<COMM: Beh.of_program (compile (add md0 (add md1 md2))) <1=
+            Beh.of_program (compile (add (add md0 md1) md2))>>
+.
+Proof.
+  ii. unfold compile in *.
+  destruct (classic (ModSem.wf (enclose (add (add md0 md1) md2)) /\ Sk.wf (sk (add (add md0 md1) md2)))).
+  2: { eapply ModSem.initial_itr_not_wf. ss. }
+  ss. des. assert (SK: Sk.wf (Sk.add (sk md0) (Sk.add (sk md1) (sk md2)))).
+  { rewrite Sk.add_assoc. apply H1. }
+  eapply ModSemFacts.add_assoc_rev; [ |et|rewrite <- Sk.add_assoc;et].
+  i. split; et. unfold enclose. ss.
+  rewrite Sk.add_assoc.
+  inv H2. inv H3. econs.
+  repeat (ss; unfold ModSem.add_fnsems in *; rewrite ! List.map_app in *; rewrite ! List.map_map in *).
+  rewrite fun_fst_trans_l in *.
+  rewrite fun_fst_trans_r in *.
+  rewrite fun_fst_trans_l_l in *.
+  rewrite fun_fst_trans_l_r in *.
+  rewrite fun_fst_trans_r_l in *.
+  rewrite fun_fst_trans_r_r in *.
+  rewrite app_assoc. apply wf_fnsems.
+Qed.
+
+Lemma add_empty_r 
+      md
+  : 
+    << EMPTY: Beh.of_program (compile (add md empty)) <1=
+              Beh.of_program (compile md)>>
+.
+Proof.
+  ii. unfold compile in *.
+  destruct (classic (ModSem.wf (enclose md) /\ Sk.wf (sk md))).
+  2: { eapply ModSem.initial_itr_not_wf. ss. }
+  ss. des. assert (SK: Sk.wf (Sk.add (sk md) Sk.unit)).
+  { rewrite Sk.add_unit_r. et.  }
+  eapply ModSemFacts.add_empty; [|et|].
+  - instantiate (1:= wf (add md empty)). i.
+    unfold wf. esplits; et. ss.
+    inv H0. econs. 
+    rewrite Sk.add_unit_r.
+    unfold ModSem.add, ModSem.add_fnsems. ss.
+    rewrite List.map_app. rewrite List.map_map.
+    ss. rewrite app_nil_r.
+    rewrite fun_fst_trans_l.
+    ss.
+
+  - unfold ModSem.compile, ModSem.empty, enclose.
+    rewrite Sk.add_unit_r in PR. et.
+Qed.
+
+Lemma add_empty_l 
+      md
+  : 
+    << EMPTY: Beh.of_program (compile (add empty md)) <1=
+              Beh.of_program (compile md)>>
+.
+Proof.
+  ii. apply add_empty_r. apply add_comm. et.
+Qed.
+
+Lemma add_empty_rev_r
+      md
+  : 
+    << EMPTY: Beh.of_program (compile md) <1=
+              Beh.of_program (compile (add md empty))>>
+.
+Proof.
+  ii. unfold compile in *.
+  destruct (classic (ModSem.wf (enclose (add md empty)) /\ Sk.wf (sk (add md empty)))).
+  2: { eapply ModSem.initial_itr_not_wf. ss. }
+  des. assert (SK: Sk.wf (sk md)).
+  { ss. rewrite Sk.add_unit_r in H1. et.  }
+
+  eapply ModSemFacts.add_empty_rev.
+  
+  2: { ss. rewrite Sk.add_unit_r in *. inv H0. econs. 
+       unfold ModSem.add in wf_fnsems. ss.
+       unfold ModSem.add_fnsems in wf_fnsems. ss.
+       rewrite List.map_app in wf_fnsems.
+       rewrite List.map_map in wf_fnsems.
+       rewrite fun_fst_trans_l in wf_fnsems. ss.
+       eapply nodup_app_l in wf_fnsems. ss. }
+  - instantiate (1:= wf md). i.
+    unfold wf. esplits; et. ss.
+    inv H0. econs. 
+    rewrite Sk.add_unit_r in wf_fnsems.
+    unfold ModSem.add, ModSem.add_fnsems in *. ss.
+    rewrite List.map_app, List.map_map in wf_fnsems.
+    ss. rewrite app_nil_r in wf_fnsems.
+    rewrite fun_fst_trans_l in wf_fnsems.
+    ss.
+
+  - unfold ModSem.compile, ModSem.empty, enclose. ss.
+    rewrite Sk.add_unit_r. et.
+Qed.
+
+Lemma add_empty_rev_l
+      md
+  : 
+    << EMPTY: Beh.of_program (compile md) <1=
+              Beh.of_program (compile (add empty md))>>
+.
+Proof. 
+  ii. apply add_comm. apply add_empty_rev_r. et. 
+Qed.
+
+
+
+(* Do we still add by list? (and refines2, refines_proper, etc.) *)
+(* Definition add_list (xs: list t): t :=
+  fold_right add empty xs
+. *)
+
+Lemma add_list_single: forall (x: t), add_list [x] = x.
+Proof. ii; cbn. refl. Qed.
+
+
+Lemma add_list_cons
+          x xs
+          (A: xs <> [])
+        :
+          (add_list (x::xs) = (add x (add_list xs)))
+.
+Proof. ss. destruct xs; ss. Qed.
+
+  Lemma add_list_sk (mdl: list t)
+  :
+    Mod.sk (add_list mdl)
+    =
+    fold_right Sk.add Sk.unit (List.map sk mdl).
+  Proof.
+    induction mdl; ss. rewrite <- IHmdl.
+    destruct mdl; ss.
+    rewrite Sk.add_unit_r. et.
+  Qed.
+
+  Fixpoint add_mrs_list (xs: list (itree coreE Any.t)): itree coreE Any.t :=
+    match xs with
+    | [] => Ret tt↑
+    | x::[] => x
+    | x::l => st1 <- x;; st2 <- (add_mrs_list l);; Ret (Any.pair st1 st2)
+    end.
+
+  (* Fixpoint add_mrs_list (xs: list Any.t): Any.t :=
+    match xs with
+    | [] => tt↑
+    | x::[] => x
+    | x::l => Any.pair x (add_mrs_list l)
+    end. *)
+
+
+  (* Lemma add_list_initial_mrs (mdl: list t) (ske: Sk.t)
+     :
+       ModSem.initial_st (Mod.get_modsem (add_list mdl) ske)
+       =
+       add_mrs_list ((List.map (fun md => ModSem.initial_st (get_modsem md ske)) mdl)).
+   Proof.
+     induction mdl; ss.
+     destruct mdl; ss.
+     rewrite <- IHmdl; ss.
+   Qed.
+
+
+  Lemma add_list_fns (mdl: list t) (ske: Sk.t)
+  :
+    List.map fst (ModSem.fnsems (Mod.get_modsem (add_list mdl) ske))
+    =
+    fold_right (@app _) [] (List.map (fun md => List.map fst (ModSem.fnsems (get_modsem md ske))) mdl).
+Proof.
+  induction mdl.
+  { auto. }
+  transitivity ((List.map fst (ModSem.fnsems (get_modsem a ske)))++(fold_right (@app _) [] (List.map (fun md => List.map fst (ModSem.fnsems (get_modsem md ske))) mdl))); auto.
+  rewrite <- IHmdl. clear.
+  ss. destruct mdl; ss. 
+  - rewrite app_nil_r. ss.
+  - unfold ModSem.add_fnsems. 
+    rewrite ! map_app. rewrite ! List.map_map.
+    rewrite fun_fst_trans_l, fun_fst_trans_r. 
+    f_equal.
+Qed. *)
+
+
+End BEH.
+End ModFacts.
